examples/CCS/OpDenot.v
@@ -3,9 +3,21 @@ From CTree Require Import
 	CTrees
 	Interp
 	Equ
-	Bisim.
+	Bisim
+  Trans.
 
-From CTreeCCS Require Import 
+From RelationAlgebra Require Import
+     monoid
+     kat
+     kat_tac
+     prop
+     rel
+     srel
+     comparisons
+     rewriting
+     normalisation.
+
+From CTreeCCS Require Import
 	Syntax
 	Denotation
 	Operational.
@@ -15,26 +27,168 @@ Import DenNotations.
 Import OpNotations.
 Open Scope ccs_scope.
 
-(*
-Definition forward (R : term -> term -> Prop) : Prop :=
-	forall P a P' Q, 
+(* Notation "t ⊢ l →sem u" := (trans l ⟦t⟧ ⟦u⟧) (at level 10) : ccs_scope. *)
+
+Lemma trans_nil_inv : forall l p, ~ trans l nil p.
+Proof.
+  intros * abs; eapply stuckV_is_stuck; apply abs.
+Qed.
+
+Definition ι : option action -> @label ccsE :=
+  fun a => match a with
+        | None => tau
+        | Some a => comm a
+        end.
+
+Definition γ : @label ccsE -> option action :=
+  fun l => match l with
+        | val x => None
+        | tau   => None
+        | obs (Act a) _ => Some a
+        end.
+
+Lemma are_opposite_op : forall a, are_opposite a (op a).
+Proof.
+  unfold op, are_opposite.
+  intros []; cbn; rewrite eqb_refl; auto.
+Qed.
+
+Lemma use_channel_can_comm : forall c a,
+  use_channel c a = false <->
+  can_comm c (ι a) = true.
+Proof.
+  unfold can_comm, use_channel.
+  intros ? [[]|]; cbn; split; auto.
+  all:match goal with |- context[if ?b then _ else _] => destruct b; easy end.
+Qed.
+
+Definition forward_func (R : term -> term -> Prop) : Prop :=
+  forall P P' Q a,
 		R P Q ->
-		P ⊢ a →op P' -> 
-	exists Q', Q ⊢ a →sem Q' /\ R P' Q'.
+		P ⊢ a →op P' ->
+	  exists Q', trans (ι a) ⟦Q⟧ ⟦Q'⟧ /\ R P' Q'.
 
-Lemma complete : exists R, forward R.
-Admitted.
+Lemma complete_func : forward_func eq.
+Proof.
+  red.
+  induction P; intros * HR TR; cbn in *.
+  - inv TR.
+  - inv TR.
+    eexists; split; [| reflexivity].
+    apply trans_TauV.
+  - inv TR.
+    eexists; split; [| reflexivity].
+    apply trans_prefix.
+  - inv TR.
+    + edestruct IHP1 as (? & ? & ?); subst; eauto.
+      eexists; split; [| reflexivity].
+      apply trans_paraL; eassumption.
+    + edestruct IHP2 as (? & ? & ?); subst; eauto.
+      eexists; split; [| reflexivity].
+      apply trans_paraR; eassumption.
+    + edestruct IHP1 as (? & trP & ?); eauto.
+      edestruct IHP2 as (? & trQ & ?); eauto.
+      subst; eexists; split; [| reflexivity].
+      eapply (trans_paraSynch trP trQ).
+      apply are_opposite_op.
+  - inv TR.
+    + edestruct IHP1 as (? & ? & ?); eauto; subst.
+      eexists; split; [| reflexivity].
+      apply trans_plusL; eassumption.
+    + edestruct IHP2 as (? & ? & ?); eauto; subst.
+      eexists; split; [| reflexivity].
+      apply trans_plusR; eassumption.
+  - inv TR.
+    edestruct IHP as (? & ? & ?); eauto; subst.
+    eexists; split; [| reflexivity].
+    apply trans_new; eauto.
+    apply use_channel_can_comm; auto.
+Qed.
 
-Definition backward (R : term -> term -> Prop) : Prop :=
-	forall P a Q Q', 
+Definition backward_func (R : term -> term -> Prop) : Prop :=
+  forall P Q Q' l,
 		R P Q ->
-		Q ⊢ a →sem Q' -> 
-	exists P', P ⊢ a →op P' /\ R P' Q'.
+    trans l ⟦Q⟧ ⟦Q'⟧ ->
+	  exists P', P ⊢ γ l →op P' /\ R P' Q'.
 
-Lemma correct : exists R, backward R.
+Lemma correct_func : backward_func (fun P Q => ⟦P⟧ ≅ ⟦Q⟧).
+Proof.
+  red; induction P; intros * HR TR;
+    cbn in *; rewrite <- HR in TR.
+  - exfalso; eapply trans_nil_inv,TR.
+  - apply trans_TauV_inv in TR as [EQ ->].
+    eexists; split; [constructor |].
+    symmetry; auto.
+  - apply trans_prefix_inv in TR as [EQ ->].
+    eexists; split; [constructor |].
+    symmetry; auto.
+  - trans_para_invT TR.
+    + (* Need to ensure that trans led to the model of someone? *)
+      (* apply IHP1 in TRp. *)
+      (* eexists; split. *)
+      (* apply SParL; eauto. *)
 Admitted.
 
-Lemma bisim : exists R, backward R /\ forward R.
+Definition forward (R : term -> ccs -> Prop) : Prop :=
+  forall P P' Q a,
+		R P Q ->
+		P ⊢ a →op P' ->
+	  exists Q', trans (ι a) Q Q' /\ R P' Q'.
+
+Definition bisim_rel := fun P q => q ≅ ⟦P⟧.
+Arguments bisim_rel/.
+
+Lemma complete : forward bisim_rel.
+Proof.
+  red.
+  induction P; intros * HR TR; cbn in *.
+  - inv TR.
+  - inv TR.
+    exists ⟦ P' ⟧.
+    split; [| reflexivity].
+    rewrite HR; apply trans_TauV.
+  - inv TR.
+    exists ⟦ P' ⟧.
+    split; [| reflexivity].
+    rewrite HR. apply trans_prefix.
+  - inv TR.
+    + edestruct IHP1 as (? & ? & EQ); eauto.
+      eexists; split.
+      rewrite HR; apply trans_paraL; eassumption.
+      rewrite EQ; reflexivity.
+    + edestruct IHP2 as (? & ? & EQ); eauto.
+      eexists; split.
+      rewrite HR; apply trans_paraR; eassumption.
+      rewrite EQ; reflexivity.
+    + edestruct IHP1 as (? & ? & EQ1); eauto.
+      edestruct IHP2 as (? & ? & EQ2); eauto.
+      eexists; split.
+      rewrite HR; eapply trans_paraSynch; cbn in *; eauto.
+      apply are_opposite_op.
+      rewrite EQ1,EQ2; reflexivity.
+  - inv TR.
+    + edestruct IHP1 as (? & ? & EQ); eauto.
+      eexists; split.
+      rewrite HR; apply trans_plusL; eassumption.
+      rewrite EQ; reflexivity.
+    + edestruct IHP2 as (? & ? & EQ); eauto.
+      eexists; split.
+      rewrite HR; apply trans_plusR; eassumption.
+      rewrite EQ; reflexivity.
+  - inv TR.
+    edestruct IHP as (? & ? & EQ); eauto.
+    eexists.
+    split.
+    rewrite HR.
+    apply trans_new; eauto.
+    apply use_channel_can_comm; auto.
+    (* Need congruence for restrict *)
+    admit.
 Admitted.
 
-*)
+Definition backward (R : term -> ccs -> Prop) : Prop :=
+  forall P Q Q' l,
+		R P Q ->
+    trans l Q Q' ->
+	  exists P', P ⊢ γ l →op P' /\ R P' Q'.
+
